proof/SimModSem.v
@@ -12,7 +12,7 @@ Require Import Values Integers.
 Require Import Globalenvs.
 Require Import Program.
 
-Require Import SimSymb Ord.
+Require Import Skeleton SimSymb Ord.
 
 Set Implicit Arguments.
 
@@ -93,7 +93,7 @@ Section SIMMODSEM.
       (* (INTERNALSRC: ms_src.(ModSem.is_internal) st_src0) *)
       (* (INTERNALTGT: ms_tgt.(ModSem.is_internal) st_tgt0) *)
       (* (SAFESRC: ms_src.(ModSem.is_step) st_src0) *)
-      (SAFESRC: ~ ms_src.(ModSem.is_call) st_src0 /\ ~ ms_src.(ModSem.is_return) st_src0)
+      (SAFESRC: ~ ms_src.(ModSem.may_call) st_src0 /\ ~ ms_src.(ModSem.is_return) st_src0)
       (FSTEP: fsim_step (lxsim sm_init) i0 st_src0 st_tgt0 sm0)
       (* Note: We used coercion on determinate_at. See final_state, which is bot2. *)
       (* sd_determ_at_final becomes nothing, but it is OK. *)
@@ -147,17 +147,19 @@ Section SIMMODSEM.
       (*     exists rs_arg_tgt m_arg_tgt, <<ATTGT: ms_tgt.(at_external) st_tgt0 rs_arg_tgt m_arg_tgt>>) *)
       (* (SAFESRC: exists rs_arg_src m_arg_src, <<ATSRC: ms_src.(at_external) st_src0 rs_arg_src m_arg_src>>) *)
       (* (SAFESRC: ms_tgt.(is_call) st_tgt0) *)
-      (SAFESRC: ms_src.(is_call) st_src0)
+      (SAFESRC: ms_src.(may_call) st_src0)
       (* (PROGSRC: ms_src.(is_call) st_src0) *)
       (CALLFSIM: forall
+          skenv_link_src skenv_link_tgt
+          (FUNCSIM: SimSymb.skenv_func_bisim sm0.(SimMem.sim_val) skenv_link_src skenv_link_tgt)
           args_src
-          (ATSRC: ms_src.(at_external) st_src0 args_src)
+          (ATSRC: ms_src.(at_external) skenv_link_src st_src0 args_src)
         ,
           exists args_tgt sm_arg,
             (<<SIMARGS: sim_args args_src args_tgt sm_arg>>
             /\ (<<MWF: SimMem.wf sm_arg>>)
             /\ (<<MLE: SimMem.le sm0 sm_arg>>)
-            /\ (<<ATTGT: ms_tgt.(at_external) st_tgt0 args_tgt>>)
+            /\ (<<ATTGT: ms_tgt.(at_external) skenv_link_tgt st_tgt0 args_tgt>>)
             /\
             (<<K: forall
                 sm_ret retv_src retv_tgt
@@ -247,7 +249,7 @@ Context {SM: SimMem.class} {SS: SimSymb.class SM}.
   (* ####################### TODO: Rename initial_machine/final_machine into initial_frame/final_frame *)
   Inductive sim (msp: t): Prop :=
   | sim_intro
-      (SIMSKENV: sim_skenv msp msp.(sm))
+      (* (SIMSKENV: sim_skenv msp msp.(sm)) *)
       (SIM: forall
           sm_arg
           args_src args_tgt
@@ -257,6 +259,7 @@ Context {SM: SimMem.class} {SS: SimSymb.class SM}.
           (FINDFTGT: msp.(tgt).(ModSem.skenv).(Genv.find_funct) args_tgt.(Args.fptr) =
                      Some (Internal sg_init_tgt))
           (SIMARGS: sim_args args_src args_tgt sm_arg)
+          (SIMSKENV: sim_skenv msp sm_arg)
           (MFUTURE: SimMem.future msp.(sm) sm_arg)
           (MWF: SimMem.wf sm_arg)
         ,
